move to new tactics; totally explicit remove function

examples/JahobAssocList.v
@@ -67,33 +67,33 @@ Module Type JAHOB_ASSOC_LIST.
  Open Scope hprop_scope.
 
  Parameter t   : Set.
- Parameter rep : list (prod K V) -> t -> hprop.
+ Parameter rep : t -> list (prod K V) -> hprop.
 
- Parameter new : STsep __ (rep nil).
+ Parameter new : STsep __ (fun r => rep r nil).
  Parameter free: forall (p: t),
-   STsep (rep nil p) (fun _: unit => __).
+   STsep (rep p nil) (fun _: unit => __).
 
  Parameter containsKey: forall k (p: t) (m: [list (prod K V)]),
-   STsep (m ~~ rep m p)
-         (fun r:bool => m ~~ rep m p * if r then Exists v :@ V, [In (k,v) m] 
+   STsep (m ~~ rep p m)
+         (fun r:bool => m ~~ rep p m * if r then Exists v :@ V, [In (k,v) m] 
                                             else [lookup m k = None]).
  (* todo: ~ Exists v, In (k,v) m] *)
 
  Parameter add: forall k v (p: t) (m: [list (prod K V)]),
-  STsep (m ~~ rep m p * [forall v, ~ In (k,v) m])
-        (fun _:unit => m ~~ rep ((k,v)::m) p).
+  STsep (m ~~ rep p m * [forall v, ~ In (k,v) m])
+        (fun _:unit => m ~~ rep p ((k,v)::m)).
 
  Parameter replace: forall k v (p: t) (m: [list (prod K V)]),
-  STsep (m ~~ rep m p * Exists v0 :@ V, [In (k,v0) m] )
-        (fun r:V => m ~~ [In (k, r) m] * rep ((k,v)::(delete m k)) p).
+  STsep (m ~~ rep p m * Exists v0 :@ V, [In (k,v0) m] )
+        (fun r:V => m ~~ [In (k, r) m] * rep p ((k,v)::(delete m k))).
 
  Parameter put: forall k v (p: t) (m: [list (prod K V)]), 
-   STsep (m ~~ rep m p)
-         (fun r => m ~~ [r = lookup m k] * rep (insert m k v) p).
+   STsep (m ~~ rep p m)
+         (fun r => m ~~ [r = lookup m k] * rep p (insert m k v)).
 
  Parameter get: forall k   (p: t) (m: [list (prod K V)]),
-   STsep (m ~~ rep m p)
-         (fun r => m ~~ rep m p * match r with
+   STsep (m ~~ rep p m)
+         (fun r => m ~~ rep p m * match r with
                                     | None => [lookup m k = None]
                                     | Some v => [In (k, v) m]
                                   end).
@@ -101,11 +101,11 @@ Module Type JAHOB_ASSOC_LIST.
 (* todo [~ Exists v @: V, In m (k, v) (maybe switch to forall v, ~ In k v ? *)
 
  Parameter isEmpty: forall (p: t) (m: [list (prod K V)]),
-   STsep (m ~~ rep m p) (fun r:bool => m ~~ rep m p * if r then [m = nil] else [m <> nil]).
+   STsep (m ~~ rep p m) (fun r:bool => m ~~ rep p m * if r then [m = nil] else [m <> nil]).
 
  Parameter remove: forall k (p: t) (m: [list (prod K V)]),
-  STsep (m ~~ rep m p * Exists v :@ V, [In (k,v) m])
-        (fun r:V => m ~~ [In (k, r) m] * rep (delete m k) p).
+  STsep (m ~~ rep p m * Exists v :@ V, [In (k,v) m])
+        (fun r:V => m ~~ [In (k, r) m] * rep p (delete m k)).
 
 (* todo: classical logic -> proof irrelevence -> inconsistency *)
 
@@ -132,102 +132,321 @@ Module JahobAssocList(A : NONDEP_ASSOCIATION) : JAHOB_ASSOC_LIST with Module A :
     next : option ptr
   }.
 
-  Fixpoint rep' m (op: option ptr) {struct m} :=
+  Fixpoint rep' (op: option ptr) m {struct m} :=
     match op with
       | None => [m = nil] 
       | Some h => match m with
                     | (k,v) :: b =>  Exists nxt :@ option ptr,
-                          h --> node k v nxt * rep' b nxt * [lookup b k = None]
+                          h --> node k v nxt * rep' nxt b * [lookup b k = None]
                     | nil => [False]
                    end
     end.
 
-  Definition rep m p : hprop :=
-    Exists n :@ option ptr, p --> n * rep' m n.
+  Definition rep p m : hprop :=
+    Exists n :@ option ptr, p --> n * rep' n m.
 
 (* Reasoning **************************************************)
 
-
- Lemma nilrep : forall m k, 
-  rep' m None ==> rep' m None * [lookup m k = None].
-   intros. destruct m. sep fail auto. simpl. assert (p :: m = nil -> False).
-   discriminate. sep fail auto. Defined.
-
- Hint Resolve nilrep.
-
- Lemma eta_node : forall fn, fn = node (key fn) (value fn) (next fn).
-   destruct fn; reflexivity.
-  Qed.
-  Hint Resolve eta_node.
-
-  Lemma eta_node2 : forall fn a b, 
-   Some (a, b) = Some (key fn, value fn) -> 
-   fn = node a b (next fn).
-    intros fn a b pf; assert (a = key fn); try congruence; 
-   assert (b = value fn); try congruence; subst; apply eta_node. 
-  Qed.
-  Hint Resolve eta_node2.
-
-  Ltac simplr := repeat (try discriminate;
+Ltac simplr := repeat (try discriminate;
   match goal with
     | [ H : head ?x = Some _ |- _ ] =>
       destruct x; simpl in *; [
         discriminate
         | injection H; clear H; intros; subst
       ]
-    | [ |- context[ match ?v with
+    | [ |- match ?v with
              | Some _ => _
-             | None   => _ 
-           end ==> _] ] => destruct v  
+             | None   => _
+           end ==> _] => destruct v
     | [ H : _ :: _ = _ :: _ |- _ ] => injection H; clear H; intros; subst
-    | [ |- context[ if (eqK ?v1 ?v2) then _ else _ ] ] => destruct (eqK v1 v2)
-    | [ H : Some ?a = Some ?b |- _ ] => assert (a = b); congruence; subst 
+    | [ H : next _ = _ |- _ ] => rewrite -> H
+    | [ H : Some _ = Some _ |- _ ] => inversion H; clear H
+    | [  H : ?a = ?b -> False , HH : (if (eqK ?a ?b) then Some _ else None) = Some _  |- _ ] => destruct (eqK a b) ; [ contradiction | discriminate ] 
+    | [  HH : (if (eqK ?a ?b) then Some _ else _) = None  |- _ ] => destruct (eqK a b) ; [ discriminate | idtac ]
+    | [  H : ?a = ?b -> False , HH : (if (eqK ?a ?b) then Some _ else Some ?v1) = Some ?v  |- context[Some ?v1 = Some ?v] ] => 
+           destruct (eqK a b) ; [ try congruence | try contradiction ] 
+    | [ _ : ?a = ?b -> False ,  HH : (if (eqK ?a ?b) then _ else ?c) = ?d  |- _ ] => destruct (eqK a b) ; [ contradiction | idtac ]
+    | [ |- context[ if eqK ?a ?a then _ else _ ] ] => destruct (eqK a a) 
+    | [ H : ?a = ?b -> False |- context[ if eqK ?a ?b then _ else _ ] ] => destruct (eqK a b); [ contradiction | idtac ] 
+    | [  H : next ?nn = ?a |- ?n = node (key ?nn) (value ?nn) ?a ] => rewrite <- H; destruct n; reflexivity
+    | [ _ : (if eqK ?a ?b then Some _ else None) = Some _ |- _ ] => destruct (eqK a b); [ idtac | discriminate ] 
+  (*  | [ |- context[ if (eqK ?v1 ?v2) then _ else _ ] ] => destruct (eqK v1 v2) *)
   end).
 
- Ltac printGoal := match goal with [ |- ?g ] => idtac g end.
+Ltac t := unfold rep; unfold rep'; sep fail simplr.
+Ltac f := fold rep'; fold rep.
 
- Ltac t := unfold rep; unfold rep'; try congruence; try subst; sep fail simplr.
- Ltac f := fold rep'; fold rep.
+Lemma eta_node : forall fn, fn = node (key fn) (value fn) (next fn).
+  destruct fn; reflexivity.
+Qed.
 
- Lemma reprev : forall hd0 m,
-   rep' m (Some hd0) ==> Exists n :@ Node,
-   [head m = Some (key n, value n)] * hd0 --> n *
-   rep' (tail m) (next n). 
- intros. destruct m. t. t. Defined.
+Hint Resolve eta_node.
 
- Lemma lkup : forall v k x, Some v = lookup x k -> In (k, v) x.
-  induction x; simpl; t. destruct a as [k0 v0]; destruct (eqK k k0); [ left; congruence | right; apply IHx; assumption ]. Qed.
-(*
- Lemma lkupNone : forall k v x,  ~ In (k, v) x -> lookup x k = None.
-  induction x; simpl; t. destruct a as [k0 v0]. destruct (eqK k k0). [ left; congruence | right; apply Ihx; assumption]. Qed.  
-*)
+Lemma ll_concat : forall nde a b c hd, Some (key nde, value nde) = head a ->
+  rep' (next nde) (tail a ++ b :: c) * hd --> nde * [lookup (tail a ++ b :: c) (key nde) = None] ==> rep' (Some hd) (a ++ b :: c)  .
+  induction a; t.
+Qed.
+
+Hint Resolve ll_concat.
+Lemma cons_nil : forall l2 x0 x, rep' l2 x0 * rep' None x ==> rep' l2 (x ++ x0).
+  destruct x; t.
+Qed.
+Lemma node_next : forall nde p,  next nde = p -> nde = node (key nde) (value nde) p.
+  destruct nde; simpl; congruence.
+Qed.
+
+Hint Resolve cons_nil.
+Hint Resolve node_next.
+
+Lemma lkup: forall m k x, 
+ lookup m x = None -> lookup (delete m k) x = None.
+  intros. induction m. trivial. simpl in *. destruct a. destruct (eqK x k0). discriminate. destruct (eqK k k0). assumption. pose (IHm H). simpl.
+  destruct (eqK x k0). subst. elim n. reflexivity. exact e. Qed.  
+
+(* Hint Resolve lkup. *)
+
+Theorem rep'_None : forall ls,
+  rep' None ls ==> [ls = nil].
+  destruct ls; sep fail idtac.
+Qed.
+
+Theorem rep'_Some : forall ls hd,
+  rep' (Some hd) ls ==> Exists k :@ K, Exists v :@ V, Exists t :@ list (prod K V), Exists p :@ option ptr,
+  [ls = (k,v) :: t] * hd --> node k v p * [lookup t k = None] * rep' p t.
+  destruct ls; sep fail ltac:(try discriminate).
+Qed.
+
+Lemma node_eta : forall fn k v x,
+  [fn = node k v x] ==> [key fn = k] * [value fn = v] * [next fn = x].
+  destruct fn; sep fail ltac:(try congruence).
+Qed.
+
+Lemma cons_eta : forall x h t,
+  [x = h :: t] ==> [head x = Some h] * [tail x = t].
+  destruct x; sep fail ltac:(try congruence).
+Qed.
+
+Lemma rep'_eq : forall m x v0 v1 x0 fn,
+  m = [x]%inhabited
+  -> (m ~~~ tail m) = [x0]%inhabited
+  -> tail x = v0
+  -> next fn = v1
+  -> rep' v1 v0 ==> rep' (next fn) x0.
+  t.
+Qed.
+
+Hint Resolve rep'_eq.
+
+Theorem rep_rep' : forall m p, rep p m ==>
+  Exists n :@ option ptr, p --> n * rep' n m. t. Qed.
+
+Hint Resolve rep_rep'.
+
+Ltac simp_prem :=
+  simpl_IfNull;
+  repeat simpl_prem ltac:(apply rep'_None || apply rep'_Some || apply node_eta || apply cons_eta || apply rep_rep');
+    unpack_conc.
+
+Ltac destr := match goal with [ x : list (prod K V) |- context[rep' None ?x] ] => destruct x; try t end.
+
+Ltac t'' := unfold rep; fold rep'; sep simp_prem simplr.
+
+Ltac t' := match goal with
+             | [ |- _ ==> ?P ] =>
+               match P with
+                 | context[rep' (next _) _] =>
+                   inhabiter; simp_prem;
+                   intro_pure; simpl_prem ltac:(solve [ eauto ]); unintro_pure; canceler; t''
+               end
+             | _ => t''
+           end.
 
 (* Implementation ***************************************************)
 
   Open Scope stsepi_scope.
 
-  Definition new : STsep __ (rep nil).
+  Definition new : STsep __ (fun r => rep r nil).
     refine {{ New (@None ptr) }}; t. Qed.
 
-  Definition free  p: STsep (rep nil p) (fun _:unit => __).
-  intros; refine {{ Free p }}; t. Qed.  
+  Definition free  p: STsep (rep p nil) (fun _:unit => __).
+  intros; refine {{ Free p }}; t. Qed.   
 
   (* This is get duplicated, so I'm going to defer until get is nicer *)
   Parameter containsKey: forall k (p: t) (m: [list (prod K V)]),
-   STsep (m ~~ rep m p)
-         (fun r:bool => m ~~ rep m p * if r then Exists v :@ V, [In (k,v) m] 
+   STsep (m ~~ rep p m)
+         (fun r:bool => m ~~ rep p m * if r then Exists v :@ V, [In (k,v) m] 
                                             else [lookup m k = None]).
 
   Definition add': forall k v (p: t) (m: [list (prod K V)]),
-   STsep (m ~~ rep m p * [lookup m k = None])
-         (fun _:unit => m ~~ rep ((k,v)::m) p).
+   STsep (m ~~ rep p m * [lookup m k = None])
+         (fun _:unit => m ~~ rep p ((k,v)::m)).
    intros. refine ( op <- ! p ;
                     n  <- New (node k v op) ;
                     {{ p ::= (Some n) }} ); t. Qed.
 
+(* Replace        **********)
+
+ Parameter replace: forall k v (p: t) (m: [list (prod K V)]),
+  STsep (m ~~ rep p m * Exists v0 :@ V, [In (k,v0) m] )
+        (fun r:V => m ~~ [In (k, r) m] * rep p ((k,v)::(delete m k))).
+
+ (* Put           *********)
+
+ Parameter put: forall k v (p: t) (m: [list (prod K V)]), 
+   STsep (m ~~ rep p m)
+         (fun r => m ~~ [r = lookup m k] * rep p (insert m k v)).
+
+ (* Get           **********)
+
+ Definition get'' (k: K) (hd: option ptr) (m: [list (prod K V)]):
+    STsep (m ~~ rep' hd m) (fun r => m ~~ [r = lookup m k] * rep' hd m).
+  intro k.
+  refine (Fix2
+    (fun hd m => m ~~ rep' hd m)
+    (fun hd m o => m ~~ [o = lookup m k] * rep' hd m)
+    (fun self hd m =>  
+      IfNull hd
+      Then  {{ Return None }}
+      Else  fn <- ! hd ;
+            if eqK k (key fn) 
+            then {{ Return (Some (value fn)) }} 
+            else {{ self (next fn) (m ~~~ tail m) <@> _ }})); t'. Qed. 
+
+  Definition get' (k: K) (p: ptr) (m: [list (prod K V)]) :
+    STsep (m ~~ rep p m)
+          (fun r:option V => m ~~ rep p m * [r = lookup m k] ).
+  intros; refine (hd <- !p;
+                  Assert (p --> hd * (m ~~ rep' hd m));;
+                  {{get'' k hd m <@> _}}); t. Qed.
+
+ (* isEmpty         ********)
+
+ Definition isEmpty: forall (p: t) (m: [list (prod K V)]),
+   STsep (m ~~ rep p m) (fun r:bool => m ~~ rep p m * if r then [m = nil] else [m <> nil]).
+   intros; refine ( ohd <- SepRead p (fun ohd => m ~~ rep' ohd m) ;
+                    IfNull ohd 
+                    Then  {{ Return true  }}
+                    Else  {{ Return false }} ); t'. Qed.
+
+ (* Remove         *********)
+
+(* t results in missing existentials whereas sep auto does not *)
+Definition removeNode  (pn: Node) (ls: list (prod K V)) (k: K) (n: Node) (prev cur: ptr) (v: V) :
+ STsep ([k = key n] * Exists t :@ list (prod K V), cur --> n * [lookup t (key pn) = None] *
+        [ls = (key pn, value pn) :: (key n, value n) :: t] * [key pn <> key n] * 
+        prev --> node (key pn) (value pn) (Some cur) * rep' (next n) t * [lookup ((key n, value n)::t) k = Some v])
+      (fun r:V =>  Exists x :@ list (prod K V), 
+                [ls = (key pn, value pn) :: x] * rep' (Some prev) ((key pn, value pn)::(delete x k)) * [r = v]).
+intros. refine (  Free cur ;;
+                  prev ::= node (key pn) (value pn) (next n) ;;  
+                  {{ Return (value n) }} ); try sep fail auto; t. Qed. 
+
+Definition recurse cur n pn nt ls prev  k v 
+(F: forall prev ls,
+               STsep(Exists pk :@ K, Exists pv :@ V, Exists ck :@ K, Exists cv :@ V,  Exists t :@ list (prod K V), Exists cur :@ ptr, Exists nxt :@ option ptr,
+               [lookup t pk = None] * [ls = (pk,pv) :: (ck, cv) :: t] * [pk <> k] * [pk <> ck] * [lookup t ck = None] *
+               prev --> node pk pv (Some cur) * cur --> node ck cv nxt  * rep' nxt t * [lookup ((ck, cv)::t) k = Some v])
+         (fun r => 
+               Exists pk :@ K, Exists pv :@ V, Exists x :@ list (prod K V), 
+               [ls = (pk,pv) :: x] * rep' (Some prev) ((pk,pv)::(delete x k)) * [r = v])) :
+STsep 
+               (Exists t :@ list (prod K V), cur --> n * [lookup t (key pn) = None] * [next pn = Some cur] * [next n = Some nt] *
+                [ls = (key pn, value pn) :: (key n, value n) :: t] * [key pn <> k] * [k <> key n] * [key pn <> key n] * [lookup t (key n) = None] *
+                 prev --> node (key pn) (value pn) (Some cur) * rep' (Some nt) t * [lookup ((key n, value n)::t) k = Some v])
+      (fun r =>  Exists x :@ list (prod K V), 
+                [ls = (key pn, value pn) :: x] * rep' (Some prev) ((key pn, value pn)::(delete x k)) * [r = v]) .
+ intros. refine ( Assert ( Exists t :@ list (prod K V), [next n = Some nt] *  [lookup t (key n) = None] * [next pn = Some cur] * 
+                           [lookup t (key pn) = None] * [k <> key pn] * [k <> key n] * cur --> n *  
+                           [key pn <> key n] *  prev --> node (key pn) (value pn) (Some cur) *
+                            [ls = (key pn, value pn) :: (key n, value n) :: t] *  rep' (Some nt) t * [lookup ((key n, value n)::t) k = Some v]) ;;
+                 {{ F cur (tail ls) <@> ( Exists t :@ list (prod K V),   [lookup t (key pn) = None] * [k <> key n] *  [k <> key pn] * [ls = (key pn, value pn) :: (key n, value n) :: t] * [lookup ((key n, value n)::t) k = Some v] * [key pn <> key n] * [next pn = Some cur] * [next n = Some nt] *  prev --> node (key pn) (value pn) (Some cur))   }}).  t. t. t'; t. clear F. sep fail auto. t. pose lkup. t. Qed.
+
+Definition remove'' k v (prev: ptr) (ls: list (prod K V)) : 
+   STsep       (Exists pk :@ K, Exists pv :@ V, Exists ck :@ K, Exists cv :@ V,  Exists t :@ list (prod K V), Exists cur :@ ptr, Exists nxt :@ option ptr,
+               [lookup t pk = None] * [ls = (pk,pv) :: (ck, cv) :: t] * [pk <> k] * [pk <> ck] * [lookup t ck = None] *
+               prev --> node pk pv (Some cur) * cur --> node ck cv nxt  * rep' nxt t * [lookup ((ck, cv)::t) k = Some v])
+         (fun r => 
+               Exists pk :@ K, Exists pv :@ V, Exists x :@ list (prod K V), 
+               [ls = (pk,pv) :: x] * rep' (Some prev) ((pk,pv)::(delete x k)) * [r = v]).
+intros k v. refine (Fix2
+(fun prev ls => (Exists pk :@ K, Exists pv :@ V, Exists ck :@ K, Exists cv :@ V,  Exists t :@ list (prod K V), Exists cur :@ ptr, Exists nxt :@ option ptr,
+              [lookup t pk = None] * [ls = (pk,pv) :: (ck, cv) :: t] * [pk <> k] * [pk <> ck] *  [lookup t ck  = None] *
+              prev --> node pk pv (Some cur) * cur --> node ck cv nxt  * rep' nxt t * [lookup ((ck, cv)::t) k = Some v]))
+ (fun prev ls r => 
+                Exists pk :@ K, Exists pv :@ V, Exists x :@ list (prod K V), 
+                [ls = (pk,pv) :: x] * rep' (Some prev) ((pk,pv)::(delete x k)) * [r = v])
+ (fun self : forall prev ls,
+               STsep(Exists pk :@ K, Exists pv :@ V, Exists ck :@ K, Exists cv :@ V,  Exists t :@ list (prod K V), Exists cur :@ ptr, Exists nxt :@ option ptr,
+               [lookup t pk = None] * [ls = (pk,pv) :: (ck, cv) :: t] * [pk <> k] * [pk <> ck] * [lookup t ck = None] *
+               prev --> node pk pv (Some cur) * cur --> node ck cv nxt  * rep' nxt t * [lookup ((ck, cv)::t) k = Some v])
+         (fun r => 
+               Exists pk :@ K, Exists pv :@ V, Exists x :@ list (prod K V), 
+               [ls = (pk,pv) :: x] * rep' (Some prev) ((pk,pv)::(delete x k)) * [r = v]) =>
+     fun prev ls =>        
+   pn <- ! prev ;
+   IfNull (next pn) As cur
+   Then {{ !!! }}
+   Else n <- SepRead cur (fun n => Exists t :@ list (prod K V), [key pn <> k] * [lookup t (key pn) = None] * [next pn = Some cur] *
+                [ls = (key pn, value pn) :: (key n, value n) :: t] * [key pn <> key n] * [lookup t (key n) = None] *
+                 prev --> node (key pn) (value pn) (Some cur) * rep' (next n) t * [lookup ((key n, value n)::t) k = Some v]); 
+        {{ match eqK k (key n) return STsep 
+               (Exists t :@ list (prod K V), cur --> n *        [key pn <> k] *[lookup t (key pn) = None] * [next pn = Some cur] *
+                [ls = (key pn, value pn) :: (key n, value n) :: t] * [key pn <> key n] * [lookup t (key n) = None] *
+                 prev --> node (key pn) (value pn) (Some cur) * rep' (next n) t * [lookup ((key n, value n)::t) k = Some v])
+      (fun r =>  Exists x :@ list (prod K V), 
+                [ls = (key pn, value pn) :: x] * rep' (Some prev) ((key pn, value pn)::(delete x k)) * [r = v]) with
+          | left _ =>  {{ removeNode pn ls k n prev cur v }}
+          | right _ => {{ match (next n) as nxt return STsep 
+               (Exists t :@ list (prod K V), cur --> n * [lookup t (key pn) = None] * [next pn = Some cur] * [next n = nxt] *
+                [ls = (key pn, value pn) :: (key n, value n) :: t] * [key pn <> k] * [k <> key n] * [key pn <> key n] * [lookup t (key n) = None] *
+                 prev --> node (key pn) (value pn) (Some cur) * rep' nxt t * [lookup ((key n, value n)::t) k = Some v])
+      (fun r =>  Exists x :@ list (prod K V), 
+                [ls = (key pn, value pn) :: x] * rep' (Some prev) ((key pn, value pn)::(delete x k)) * [r = v]) with
+        | None => {{ !!! }} 
+        | Some nt =>  recurse cur n pn nt ls prev  k v self
+          end  }} end }} )). t. t. t. t. t. t. t. t. t; f; destr. t. t. t. t. t. Qed.  
+
+ Definition remove' : forall k v (p: t) (m: list (prod K V)),
+                     STsep (                        [lookup m k = Some v] * rep p m) 
+                         (fun r:V =>                [lookup m k = Some r] * rep p (delete m k)).
+ intros. refine ( 
+  ohdptr <- SepRead p (fun n => [lookup m k = Some v] * rep' n m) ;
+  match ohdptr as ohdptr return STsep ([lookup m k = Some v] * p --> ohdptr * rep' ohdptr m)
+                             (fun r => [lookup m k = Some r] * rep p (delete m k))  with
+   | None => {{ !!! }} 
+   | Some hdptr => hd <- SepRead hdptr (fun hd => Exists tl :@ list (prod K V), p --> Some hdptr * [lookup m k = Some v] *
+                          [m = (key hd, value hd)::tl] * rep' (next hd) tl * [lookup tl (key hd) = None]) ;
+
+          match eqK k (key hd) return STsep ( Exists tl :@ list (prod K V), p --> Some hdptr * [lookup m k = Some v] * hdptr --> hd *
+                                              [m = (key hd, value hd)::tl] * rep' (next hd) tl * [lookup tl (key hd) = None])
+                                 (fun r:V => [lookup m k = Some r] * rep p (delete m k)) with
+            | left _  => Free hdptr ;;
+                         p ::= next hd ;; 
+                         {{ Return (value hd) }}
+            | right _ => {{ match next hd as nxt return STsep (Exists tl :@ list (prod K V), [next hd = nxt] *  p --> Some hdptr * [lookup m k = Some v] * hdptr --> hd *
+                                              [m = (key hd, value hd)::tl] * rep' nxt tl * [lookup tl (key hd) = None])
+                                 (fun r:V => [lookup m k = Some r] * rep p (delete m k)) with
+                           | None => {{ !!! }}
+                           | Some nt => 
+Assert (
+Exists ck :@ K, Exists cv :@ V, Exists t :@ list (prod K V),  Exists nn :@ option ptr,
+p --> Some hdptr * [lookup m k = Some v] * hdptr --> hd * [Some nt = next hd] * 
+[m = (key hd, value hd)::(ck, cv)::t] * [next hd = Some nt] * nt --> node ck cv nn * rep' nn t * [lookup t ck = None] * 
+                                            [lookup ((ck, cv)::t) (key hd) = None]);; 
+                            {{ remove'' k v hdptr m <@> (Exists ck :@ K, Exists cv :@ V, Exists t :@ list (prod K V), 
+                                                        [m = (key hd, value hd)::(ck, cv)::t] * [next hd = Some nt] * 
+                                                        p --> Some hdptr * [lookup m k = Some v] * [Some nt = next hd] *
+                                                        [lookup t ck = None] *   [lookup ((ck, cv)::t) (key hd) = None]) }}  
+                         end }}
+          end
+  end). t. t. t'. t'. t'. t. t. t. t'. t'. t'. t. t. t. t. t'. t'. t. t. t'. t.  Qed.  
+        
+
+(* Equivalence to Jahob interface *)
+
   Definition add: forall k v (p: t) (m: [list (prod K V)]),
-  STsep (m ~~ rep m p * [forall v0, ~ In (k,v0) m])
-        (fun _:unit => m ~~ rep ((k,v)::m) p). 
+  STsep (m ~~ rep p m * [forall v0, ~ In (k,v0) m])
+        (fun _:unit => m ~~ rep p ((k,v)::m)). 
   intros. refine ( {{ add' k v p m }}). hdestruct m. t. sep fail auto.
    destruct (eqK k a). pose (H b). destruct f. subst. left. reflexivity.
                        induction m. t. destruct a0. simpl. destruct (eqK k k0).
@@ -235,136 +454,19 @@ Module JahobAssocList(A : NONDEP_ASSOCIATION) : JAHOB_ASSOC_LIST with Module A :
     intros. destruct H0. assert (a = k). congruence. subst. elim n. reflexivity.
     pose (H v1). destruct f. right. simpl. right. assumption. t. Qed.
 
-(* Replace        **********)
-
- Parameter replace: forall k v (p: t) (m: [list (prod K V)]),
-  STsep (m ~~ rep m p * Exists v0 :@ V, [In (k,v0) m] )
-        (fun r:V => m ~~ [In (k, r) m] * rep ((k,v)::(delete m k)) p).
-
- (* Put           *********)
-
- Parameter put: forall k v (p: t) (m: [list (prod K V)]), 
-   STsep (m ~~ rep m p)
-         (fun r => m ~~ [r = lookup m k] * rep (insert m k v) p).
-
- (* Get           **********)
-
-  Definition get'' (k: K) (hd: option ptr) (m: [list (prod K V)]):
-    STsep (m ~~ rep' m hd) (fun r => m ~~ [r = lookup m k] * rep' m hd).
-  intro k.
-  refine (Fix2
-    (fun hd m => m ~~ rep' m hd)
-    (fun hd m o => m ~~ [o = lookup m k] * rep' m hd)
-    (fun self : forall hd m, STsep (m ~~ rep' m hd) (fun r => m ~~ [r = lookup m k] * rep' m hd) => fun hd m => 
-      IfNull hd
-      Then  Assert (m ~~ [m = nil]) ;;
-            {{ Return None }}
-      Else  fn <- SepRead hd (fun fn => m ~~  [head m = Some (key fn, value fn)] * 
-                                              rep' (tail m) (next fn) *
-                                              [lookup (tail m) (key fn) = None] *
-                                              [lookup m (key fn) = Some (value fn)] );
-            if eqK (key fn) k 
-            then {{ Return (Some (value fn)) 
-                     <@>              (hd --> fn * (m ~~ 
-                                              [head m = Some (key fn, value fn)] * 
-                                              rep' (tail m) (next fn)  *
-                                              [lookup (tail m) (key fn) = None] *    
-                                              [lookup m k = Some (value fn)] ))  }}  
-            else {{ self (next fn) (m ~~~ tail m) 
-                     <@>             (hd --> fn * (m ~~  
-                                              [head m = Some (key fn, value fn)] * 
-                                              [lookup (tail m) (key fn) = None] )) }} ));
-  try solve [ t | repeat (hdestruct m; t) ]. Qed.
-
-  Definition get' (k: K) (p: ptr) (m: [list (prod K V)]) :
-    STsep (m ~~ rep m p)
-          (fun r:option V => m ~~ rep m p * [r = lookup m k] ).
-  intros; refine (hd <- !p;
-                  Assert (p --> hd * (m ~~ rep' m hd));;
-                  {{get'' k hd m <@> _}}); t. Qed.
-
-  Definition get: forall k   (p: t) (m: [list (prod K V)]),
-   STsep (m ~~ rep m p)
-         (fun r => m ~~ rep m p * match r with
+  Parameter get: forall k   (p: t) (m: [list (prod K V)]),
+   STsep (m ~~ rep p m)
+         (fun r => m ~~ rep p m * match r with
                                     | None => [lookup m k = None]
                                     | Some v => [In (k, v) m]
                                   end).
-  intros; refine ( {{ get' k p m }} ); [ t | intro v; destruct v; pose lkup; t ]. Qed.
-
- (* isEmpty         ********)
-
- Definition isEmpty: forall (p: t) (m: [list (prod K V)]),
-   STsep (m ~~ rep m p) (fun r:bool => m ~~ rep m p * if r then [m = nil] else [m <> nil]).
- intros; refine ( ohd <- ! p ;
-                   Assert (m ~~ p --> ohd * rep' m ohd) ;;
-                  {{ Return (match ohd with | None => true | Some _ => false end) }} );
- solve [ t | hdestruct m; t ]. Qed.
-
- (* Remove         *********)
+(* 
+  intros; refine ( {{ get' k p m }} ).  [ t | intro v; destruct v; pose lkup; t ]. Qed. *)
 
  Parameter remove: forall k (p: t) (m: [list (prod K V)]),
-  STsep (m ~~ rep m p * Exists v :@ V, [In (k,v) m])
-        (fun r:V => m ~~ [In (k, r) m] * rep (delete m k) p).
-
-Parameter ff: False.
-
-Definition cmp n m v k cur prev pn : STsep ([next pn = Some cur] * [key n = k] * [lookup m (key pn) = None] * cur --> n * [lookup m k = Some v] * [lookup (tail m) (key n) = None] * [head m = Some (key n, value n)] * prev --> pn * rep' (tail m) (next n))
-                                     (fun r:V => [next pn = Some cur] * [lookup m (key pn) = None] * [Some r = lookup m k] * rep' ((key pn, value pn)::(delete m k)) (Some prev)).
- intros. refine ( Free cur ;; prev ::= node (key pn) (value pn) (next n) ;; {{ Return (value n) }} ). t. t. t. t. t. t. Defined.
-
-Definition remove'' k v (prev: ptr) (pn: Node) (m: list (prod K V)) : STsep
-   ( Exists ck :@ K, Exists cv :@ V, [lookup m (key pn) = None] * [lookup m k = Some v] * [head m = Some (ck, cv)] * prev --> pn * rep' m (next pn) )
-   (fun r:V => [lookup m (key pn) = None] * [Some r = lookup m k] * rep' ((key pn, value pn)::(delete m k)) (Some prev)).
-intros k v. refine (Fix3 (fun prev pn m => Exists ck :@ K, Exists cv :@ V,  [lookup m (key pn) = None] * [lookup m k = Some v] * [head m = Some (ck, cv)] * prev --> pn * rep' m (next pn) )
-                         (fun prev pn m r => [lookup m (key pn) = None] * [Some r = lookup m k] * rep' ((key pn, value pn)::(delete m k)) (Some prev))
-                         (fun F prev (pn: Node) m => 
-{{  match next pn as nxt return STsep ([next pn = nxt] * Exists ck :@ K, Exists cv :@ V,  [lookup m (key pn) = None] * [lookup m k = Some v] * [head m = Some (ck, cv)] * prev --> pn * rep' m nxt)
-                                   (fun r:V => [next pn = nxt] * [lookup m (key pn) = None] * [Some r = lookup m k] * rep' ((key pn, value pn)::(delete m k)) (Some prev)) with
-   | None => {{ !!! }}
-   | Some cur => Assert (Exists n :@ Node,   [next pn = Some cur] * cur --> n *  [lookup m (key pn) = None] * [lookup m k = Some v] * [lookup (tail m) (key n) = None] * [head m = Some (key n, value n)] * prev --> pn * rep' (tail m) (next n)) ;; 
-                 n <- ! cur ;
-                 match eqK (key n) k as eqx return STsep ([next pn = Some cur] * match eqx with
-                                                            | left  _ => [key n  = k] 
-                                                            | right _ => [key n <> k] 
-                                                              end  * [lookup m (key pn) = None] * cur --> n  * [lookup m k = Some v] * [lookup (tail m) (key n) = None] * [head m = Some (key n, value n)] * prev --> pn * rep' (tail m) (next n))
-                                            (fun r:V => [next pn = Some cur] * [lookup m (key pn) = None] * [Some r = lookup m k] * rep' ((key pn, value pn)::(delete m k)) (Some prev)) with
-                   | left _ =>  cmp n m v k cur prev pn   
-                   | right _ => {{ match next n as nxt return STsep ([next pn = Some cur] * [next n = nxt] * [key n <> k] * [lookup m (key pn) = None] * cur --> n  * [lookup m k = Some v] * [lookup (tail m) (key n) = None] * [head m = Some (key n, value n)] * prev --> pn * rep' (tail m) nxt)
-                                            (fun r:V => [next pn = Some cur] * [lookup m (key pn) = None] * [Some r = lookup m k] * rep' ((key pn, value pn)::(delete m k)) (Some prev)) with
-                                  | None => {{ !!! }} 
-                                  | Some p => False_rect _ ff (* {{ F cur n (tail m) <@>  [next pn = Some cur] * [next n = Some p] * [key n <> k] * [lookup m (key pn) = None] * prev --> pn }} *) 
-                                 end }}
-                 end 
- end }})).  
- solve [ t | destruct m; t; destruct m; t ] . 
- solve [ t | destruct m; t; destruct m; t ] .
- solve [ t | destruct m; t; destruct m; t ] .
- solve [ t | destruct m; t; destruct m; t ] .
- solve [ t | destruct m; t; destruct m; t ] .
- solve [ t | destruct m; t; destruct m; t ] .
- solve [ t | destruct m; t; destruct m; t ] .
- solve [ t | destruct m; t; destruct m; t ] .
- solve [ t | destruct m; t; destruct m; t ] .
- solve [ t | destruct m; t; destruct m; t ] .
- solve [ t | destruct m; t; destruct m; t ] .
- solve [ t | destruct m; t; destruct m; t ] . Qed.
-
- Definition remove' : forall k v (p: t) (m: list (prod K V)),
-                     STsep (                        [lookup m k = Some v] * rep m p) 
-                         (fun r:V =>                [lookup m k = Some r] * rep (delete m k) p).
- intros. refine ( 
- ohdptr <- ! p ;
- match ohdptr with
-   | None => {{ !!! }}
-   | Some hdptr => hd <- ! hdptr ;
-                   match eqK (key hd) k with
-                     | left _  => p ::= None ;;
-                                  {{ Return (value hd) }}
-                     | right _ => {{ remove'' k v hdptr hd (tail m) }} 
-                   end
- end). Admitted.
-
-                
+  STsep (m ~~ rep p m * Exists v :@ V, [In (k,v) m])
+        (fun r:V => m ~~ [In (k, r) m] * rep p (delete m k)).
+  (* need to get witness *)
 
  (* The Jahob put operation traverses the list several times.  
     This implements a faster, in-place put that isn't found in Jahob. *)
